stdlib/lampe/Stdlib/TraitMethods.lean
@@ -1,4 +1,4 @@
-import «std-1.0.0-beta.12».Extracted
+import «std-1.0.0-beta.14».Extracted
 import Lampe
 
 /-!
@@ -12,7 +12,7 @@ pulled out into a separate file. This is that file.
 
 namespace Lampe.Stdlib
 
-open «std-1.0.0-beta.12»
+open «std-1.0.0-beta.14»
 open Lampe.Stdlib
 
 namespace Append
@@ -20,33 +20,33 @@ namespace Append
 /-- A shorthand for a call to the `std::append::Append::empty` method. -/
 @[reducible]
 def empty {p}
-    (generics : HList Kind.denote «std-1.0.0-beta.12::append::Append».«#genericKinds»)
+    (generics : HList Kind.denote «std-1.0.0-beta.14::append::Append».«#genericKinds»)
     (Self : Tp)
-    (associatedTypes : HList Kind.denote «std-1.0.0-beta.12::append::Append».«#associatedTypesKinds»)
-    (fnGenerics : HList Kind.denote «std-1.0.0-beta.12::append::Append».«#genericKinds»)
+    (associatedTypes : HList Kind.denote «std-1.0.0-beta.14::append::Append».«#associatedTypesKinds»)
+    (fnGenerics : HList Kind.denote «std-1.0.0-beta.14::append::Append».«#genericKinds»)
   : HList (Tp.denote p)
-      («std-1.0.0-beta.12::append::Append».empty.«#inputs» generics Self associatedTypes fnGenerics)
+      («std-1.0.0-beta.14::append::Append».empty.«#inputs» generics Self associatedTypes fnGenerics)
   → Expr (Tp.denote p)
-      («std-1.0.0-beta.12::append::Append».empty.«#output» generics Self associatedTypes fnGenerics) :=
-  «std-1.0.0-beta.12::append::Append».empty generics Self associatedTypes fnGenerics
+      («std-1.0.0-beta.14::append::Append».empty.«#output» generics Self associatedTypes fnGenerics) :=
+  «std-1.0.0-beta.14::append::Append».empty generics Self associatedTypes fnGenerics
 
 /-- A shorthand for a call to the `std::append::Append::append` method. -/
 @[reducible]
 def append {p}
-    (generics : HList Kind.denote «std-1.0.0-beta.12::append::Append».«#genericKinds»)
+    (generics : HList Kind.denote «std-1.0.0-beta.14::append::Append».«#genericKinds»)
     (Self : Tp)
-    (associatedTypes : HList Kind.denote «std-1.0.0-beta.12::append::Append».«#associatedTypesKinds»)
-    (fnGenerics : HList Kind.denote «std-1.0.0-beta.12::append::Append».«#genericKinds»)
+    (associatedTypes : HList Kind.denote «std-1.0.0-beta.14::append::Append».«#associatedTypesKinds»)
+    (fnGenerics : HList Kind.denote «std-1.0.0-beta.14::append::Append».«#genericKinds»)
   : HList (Tp.denote p)
-      («std-1.0.0-beta.12::append::Append».append.«#inputs» generics Self associatedTypes fnGenerics)
+      («std-1.0.0-beta.14::append::Append».append.«#inputs» generics Self associatedTypes fnGenerics)
   → Expr (Tp.denote p)
-      («std-1.0.0-beta.12::append::Append».append.«#output» generics Self associatedTypes fnGenerics) :=
-  «std-1.0.0-beta.12::append::Append».append generics Self associatedTypes fnGenerics
+      («std-1.0.0-beta.14::append::Append».append.«#output» generics Self associatedTypes fnGenerics) :=
+  «std-1.0.0-beta.14::append::Append».append generics Self associatedTypes fnGenerics
 
 /--
 Asserts that the provided `tp` has an implementation of `std::append::Append` in the environment.
 -/
 @[reducible]
-def hasImpl (env : Env) (tp : Tp) := «std-1.0.0-beta.12::append::Append».hasImpl env h![] tp
+def hasImpl (env : Env) (tp : Tp) := «std-1.0.0-beta.14::append::Append».hasImpl env h![] tp
 
 end Append
