stdlib/lampe/Stdlib/Panic.lean
@@ -1,9 +1,9 @@
-import «std-1.0.0-beta.12».Extracted
+import «std-1.0.0-beta.14».Extracted
 import Lampe
 
 namespace Lampe.Stdlib.Panic
 
-open «std-1.0.0-beta.12»
+open «std-1.0.0-beta.14»
 
 /--
 Note that this theorem exists only to make it easy to steps through calls to `panic` in your code as
@@ -11,7 +11,7 @@ it cannot (and does not) assert any meaningful properties on the functioning of 
 -/
 theorem panic_correct {p T U N msg}
   : STHoare p env ⟦⟧
-    («std-1.0.0-beta.12::panic::panic».call h![T, U, N] h![msg])
+    («std-1.0.0-beta.14::panic::panic».call h![T, U, N] h![msg])
     (fun _ => ⟦⟧) := by
   enter_decl
   steps
